theories/Common.v
@@ -6,6 +6,8 @@ From ExtLib Require Export
 From Coq Require Export
      Basics
      List.
+Export
+  ListNotations.
 Open Scope program_scope.
 
 Definition get' {K V} (eqb : K -> K -> bool) (k : K) : list (K * V) -> option V :=
@@ -13,3 +15,13 @@ Definition get' {K V} (eqb : K -> K -> bool) (k : K) : list (K * V) -> option V 
 
 Definition get {K V} `{Dec_Eq K} : K -> list (K * V) -> option V :=
   get' (fun k k' => k = k'?).
+
+Definition map_snd {K V U} (f : V -> U) : list (K * V) -> list (K * U) :=
+  map (fun kv => let (k, v) := kv : K * V in (k, f v)).
+
+Fixpoint pick_some {A} (l : list (option A)) : list A :=
+  match l with
+  | [] => []
+  | Some a :: l' => a :: pick_some l'
+  | None   :: l' =>     pick_some l'
+  end.
